Port until MP example

promise_free/system/SystemA.v
@@ -5,26 +5,26 @@ From iris.algebra Require Export csum gmap_view.
 From iris.bi Require Export fractional.
 
 Class sysG `{!crisG Γ Σ α β τ _S _I} := {
-  sys_inG :: inG (gmap_viewUR Ident.t (agreeR TViewO)) Γ
+  sys_inG :: inG (gmap_viewUR Ident.t (agreeR (TViewO * natO)%type)) Γ
 }.
 
 Section SystemRA.
-  Context `{!crisG Γ Σ α β τ _S _I, !histG, !atomicG, !sysG}.
+  Context `{!crisG Γ Σ α β τ _S _I, !concG, !histG, !atomicG, !sysG}.
 
-  Definition tview_sys_auth (ths : gmap Ident.t TView.t) : iProp Σ :=
+  Definition tview_sys_auth (ths : gmap Ident.t (TView.t * nat)) : iProp Σ :=
     (own base_γ (gmap_view_auth (DfracOwn 1) (to_agree <$> ths)) ∗
-    [∗ map] tid ↦ 𝓥 ∈ ths, tview tid 𝓥).
+    [∗ map] tid ↦ '(V, _) ∈ ths, tview tid V).
 
-  Definition tview_sys_gen (q : Qp) (tid : Ident.t) (𝓥 : TView.t) : iProp Σ :=
-    own base_γ (gmap_view_frag tid (DfracOwn q) (to_agree 𝓥)).
+  Definition tview_sys_gen (q : Qp) (mtid : Ident.t) (stid : nat) (V : TView.t) : iProp Σ :=
+    own base_γ (gmap_view_frag mtid (DfracOwn q) (to_agree (V, stid))).
+  Definition tview_sys (tid : Ident.t) (stid : nat) (V : TView.t) : iProp Σ :=
+    (tview_sys_gen 1 tid stid V ∗ TID stid ∗ YIELD stid)%I.
 
-  Definition tview_sys (tid : Ident.t) (𝓥 : TView.t) : iProp Σ :=
-    tview_sys_gen 1 tid 𝓥.
-
-  Lemma tview_sys_lookup (ths : gmap Ident.t TView.t) (tid : Ident.t) (𝓥 : TView.t) (q : Qp) :
+  Lemma tview_sys_lookup
+      (ths : gmap Ident.t (TView.t * nat)) (tid : Ident.t) (stid : nat) (𝓥 : TView.t) (q : Qp) :
     tview_sys_auth ths -∗
-    tview_sys_gen q tid 𝓥 -∗
-    ⌜ ths !! tid = Some 𝓥 ⌝.
+    tview_sys_gen q tid stid 𝓥 -∗
+    ⌜ ths !! tid = Some (𝓥, stid) ⌝.
   Proof.
     rewrite /tview_sys_auth /tview_sys /tview_sys_gen; iIntros "[TA TVS] TV".
     iCombine "TA TV" gives %[𝓥' [? [_ [Hlookup [_ Hincl]]]]]%gmap_view_both_dfrac_valid_discrete.
@@ -33,86 +33,86 @@ Section SystemRA.
     rewrite Some_included_total to_agree_included_L in Hincl; subst; done.
   Qed.
 
-  Instance tview_sys_gen_fractional tid 𝓥 : Fractional (λ q, tview_sys_gen q tid 𝓥).
+  Instance tview_sys_gen_fractional tid stid V : Fractional (λ q, tview_sys_gen q tid stid V).
   Proof. ii; by rewrite /tview_sys_gen -own_op -gmap_view_frag_add agree_idemp. Qed.
 
-  #[global] Instance tview_sys_gen_as_fractional tid 𝓥 q :
-    AsFractional (tview_sys_gen q tid 𝓥) (λ q, tview_sys_gen q tid 𝓥) q.
+  #[global] Instance tview_sys_gen_as_fractional tid stid V q :
+    AsFractional (tview_sys_gen q tid stid V) (λ q, tview_sys_gen q tid stid V) q.
   Proof. split; ss; typeclasses eauto. Qed.
 End SystemRA.
 
 Module SystemA. Section SystemA.
-  Context `{!crisG Γ Σ α β τ _S _I, !histG, !atomicG, !sysG}.
+  Context `{!crisG Γ Σ α β τ _S _I, !concG, !histG, !atomicG, !sysG}.
   Context (sp_user : spl_type).
 
   (* Specifications *)
   Definition fspec_spawnable (fn : string) (pre : TView.t → SAny.t → SAny.t → iProp Σ) : Prop :=
     ∃ fsp, alist_find (Some fn) sp_user = Some (Some fsp) ∧
-      fspec_imply
+      fspec_imply'
         fsp
         (fspec_winv ⊤
-          (fspec_virtual (λ '(tid, V),
+          (fspec_virtual (λ '(tid, stid, V),
             ((λ (varg : SAny.t) (arg : Any.t),
-              tview_sys tid V ∗ ∃ sarg, ⌜arg = sarg↑⌝ ∗ pre V varg sarg),
-            (λ (vret : SAny.t) _, tview_sys tid V)))))%I.
+              tview_sys tid stid V ∗ ∃ sarg, ⌜arg = sarg↑⌝ ∗ pre V varg sarg),
+            (λ (vret : SAny.t) _, tview_sys tid stid V)))))%I.
 
   Definition _spawn_spec : fspec := 
-    fspec_virtual (λ (_ : ()),
-      (λ varg arg,
+    fspec_spawn
+      (λ '((stid, _) : _ * ()) varg arg,
         ∃ (tid : Ident.t) V pre fvarg farg fn,
-          ⌜varg = (tid, fn, fvarg) ∧ arg = (tid, fn, farg)↑ ∧ fspec_spawnable fn pre⌝ ∗
-          tview_sys_gen (1/2) tid V ∗
-          pre V fvarg farg,
-      λ (_ : SAny.t) _, False%I))%I.
+          ⌜varg = (tid, fn, fvarg)↑ ∧ arg = (tid, fn, farg)↑ ∧ fspec_spawnable fn pre⌝ ∗
+          tview_sys_gen 1 tid stid V ∗
+          pre V fvarg farg)%I
+      (λ _ vret _, ∃ (vr : SAny.t), ⌜vret = vr↑⌝ ∗ False)%I.
 
   Definition spawn_spec (E : coPset) : fspec :=
     fspec_winv E
-      (fspec_virtual (λ '(tid, pre, 𝓥),
+      (fspec_virtual (λ '(tid, stid, pre, 𝓥),
         ((λ varg arg,
           ∃ fvarg farg fn, ⌜varg = (fn, fvarg) ∧ arg = (fn, farg)↑ ∧ fspec_spawnable fn pre⌝ ∗
-            tview_sys tid 𝓥 ∗ pre 𝓥 fvarg farg),
-        (λ vret ret, tview_sys tid 𝓥 ∗ ⌜vret = tt ∧ ret = tt↑⌝))))%I.
+            tview_sys tid stid 𝓥 ∗ pre 𝓥 fvarg farg),
+        (λ vret ret, tview_sys tid stid 𝓥 ∗ ⌜vret = tt ∧ ret = tt↑⌝))))%I.
 
   Definition yield_spec (E : coPset) : fspec :=
     fspec_winv E
-      (fspec_simple (λ '(tid, 𝓥),
-        ((λ varg, ⌜varg = tt↑⌝ ∗ tview_sys tid 𝓥),
-        (λ vret, ⌜vret = tt↑⌝ ∗ tview_sys tid 𝓥))))%I.
+      (fspec_simple (λ '(tid, stid, 𝓥),
+        ((λ varg, ⌜varg = tt↑⌝ ∗ tview_sys tid stid 𝓥),
+        (λ vret, ⌜vret = tt↑⌝ ∗ tview_sys tid stid 𝓥))))%I.
 
   Definition get_tid_spec : fspec :=
-    fspec_simple (λ '(tid, 𝓥),
-      ((λ varg, ⌜varg = tt↑⌝ ∗ tview_sys tid 𝓥),
-       (λ vret, ⌜vret = tid↑⌝ ∗ tview_sys tid 𝓥)))%I.
+    fspec_simple (λ '(tid, stid, 𝓥),
+      ((λ varg, ⌜varg = tt↑⌝ ∗ tview_sys tid stid 𝓥),
+       (λ vret, ⌜vret = tid↑⌝ ∗ tview_sys tid stid 𝓥)))%I.
 
   Definition alloc_spec : fspec :=
-    fspec_simple (X := Ident.t * nat * TView.t)
-      (λ '(tid, sz, 𝓥),
-        ((λ varg, ⌜varg = sz↑⌝ ∗ tview_sys tid 𝓥),
+    fspec_simple (X := Ident.t * nat * nat * TView.t)
+      (λ '(tid, stid, sz, 𝓥),
+        ((λ varg, ⌜varg = sz↑⌝ ∗ tview_sys tid stid 𝓥),
         (λ vret, ∃ loc 𝓥', ⌜vret = (Val.Vptr loc)↑ ∧ TView.le 𝓥 𝓥'⌝ ∗
-          tview_sys tid 𝓥' ∗
+          tview_sys tid stid 𝓥' ∗
           †loc…sz ∗
           @{TView.cur 𝓥'} loc ↦∗ repeat Val.Vundef sz)))%I.
 
   (* non-atomic read *)
   Definition read_spec_0 : fspec :=
-    fspec_simple (X:=Ident.t * Loc.t * Ordering.t * Val.t * Qp * TView.t)
-      (λ '(tid, loc, ord, v, q, 𝓥),
+    fspec_simple (X:=Ident.t * nat * Loc.t * Ordering.t * Val.t * Qp * TView.t)
+      (λ '(tid, stid, loc, ord, v, q, V),
         ((λ varg, ⌜varg = (loc, ord)↑⌝ ∗
-          @{TView.cur 𝓥} loc ↦{q} v ∗ tview_sys tid 𝓥),
-         (λ vret, ∃ v' 𝓥', ⌜vret = v'↑ ∧ Val.le v' v⌝ ∗
-          @{TView.cur 𝓥'} loc ↦{q} v ∗ tview_sys tid 𝓥')))%I.
+          @{TView.cur V} loc ↦{q} v ∗ tview_sys tid stid V),
+         (λ vret, ∃ v' V', ⌜vret = v'↑ ∧ Val.le v' v⌝ ∗
+          @{TView.cur V'} loc ↦{q} v ∗ tview_sys tid stid V')))%I.
 
   (* atomic read *)
   (* TODO : give variants of this specification (SW, SYNC, CAS, ...) *)
   Definition read_spec_1 : fspec :=
     fspec_simple
-      (X:=Ident.t * Loc.t * Ordering.t * Cell.t * Cell.t * Time.t * positive * Qp * AtomicMode * TView.t * View.t)
-      (λ '(tid, loc, ord, ζ, ζ', t, γ, q, mode, 𝓥, Vb),
+      (X:=Ident.t * nat * Loc.t * Ordering.t * Cell.t * Cell.t * Time.t * positive * Qp * AtomicMode * TView.t * View.t)
+      (λ '(tid, stid, loc, ord, ζ, ζ', t, γ, q, mode, 𝓥, Vb),
         ((λ varg,
           ⌜varg = (loc, ord)↑ ∧ Ordering.le Ordering.relaxed ord⌝ ∗
           @{TView.cur 𝓥} loc sn⊒{γ} ζ' ∗ (* ζ' abstract history seen by current thread *)
           @{Vb} AtomicPtsToX loc γ t ζ mode ∗ (* ζ global abstract history *)
-          tview_sys tid 𝓥), (* 𝓥 current thread view *)
+          tview_sys tid stid 𝓥), (* 𝓥 current thread view *)
         (λ vret, ∃ ζ'' f' na v' v'' V' 𝓥',
           ⌜vret = v'↑ ∧
           Val.le v' v'' ∧
@@ -123,18 +123,18 @@ Module SystemA. Section SystemA.
           V' ⊑ (if Ordering.le Ordering.acqrel ord then TView.cur 𝓥' else TView.acq 𝓥')⌝ ∗
           @{TView.cur 𝓥'} loc sn⊒{γ} ζ'' ∗
           @{Vb} AtomicPtsToX loc γ t ζ mode ∗
-          tview_sys tid 𝓥')))%I.
+          tview_sys tid stid 𝓥')))%I.
 
   Definition read_spec : fspec := app_fspec [read_spec_0; read_spec_1].
 
   (* non-atomic write *)
   Definition write_spec_0 : fspec :=
-    fspec_simple (X:=Ident.t * Loc.t * Val.t * Ordering.t * TView.t)
-      (λ '(tid, loc, val, ord, 𝓥),
+    fspec_simple (X:=Ident.t * nat * Loc.t * Val.t * Ordering.t * TView.t)
+      (λ '(tid, stid, loc, val, ord, V),
         ((λ varg, ⌜varg = (loc, val, ord)↑⌝ ∗
-          @{TView.cur 𝓥} loc ↦ ? ∗ tview_sys tid 𝓥),
-        (λ vret, ∃ 𝓥', ⌜vret = Val.zero↑ ∧ TView.le 𝓥 𝓥'⌝ ∗
-          @{TView.cur 𝓥'} loc ↦ val ∗ tview_sys tid 𝓥')))%I.
+          @{TView.cur V} loc ↦ ? ∗ tview_sys tid stid V),
+        (λ vret, ∃ V', ⌜vret = Val.zero↑ ∧ TView.le V V'⌝ ∗
+          @{TView.cur V'} loc ↦ val ∗ tview_sys tid stid V')))%I.
 
   #[local] Definition own_writer γ (m : AtomicMode) (q : frac) ζ tx : iProp Σ :=
     match m with
@@ -146,13 +146,13 @@ Module SystemA. Section SystemA.
   (* atomic write *)
   Definition write_spec_1 : fspec :=
     fspec_simple
-      (X:=Ident.t * Loc.t * Val.t * Ordering.t * TView.t * gname * Cell.t * View.t * Time.t * Cell.t * AtomicMode * Qp * Time.t)
-      (λ '(tid, loc, val, ord, 𝓥, γ, ζ', Vb, tx, ζ, mode, q, tx'),
+      (X:=Ident.t * nat * Loc.t * Val.t * Ordering.t * TView.t * gname * Cell.t * View.t * Time.t * Cell.t * AtomicMode * Qp * Time.t)
+      (λ '(tid, stid, loc, val, ord, 𝓥, γ, ζ', Vb, tx, ζ, mode, q, tx'),
         ((λ varg,
           ⌜varg = (loc, val, ord)↑ ∧ Ordering.le Ordering.relaxed ord⌝ ∗
           @{TView.cur 𝓥} loc sn⊒{γ} ζ' ∗
           @{Vb} AtomicPtsToX loc γ tx ζ mode ∗
-          tview_sys tid 𝓥 ∗
+          tview_sys tid stid 𝓥 ∗
           own_writer γ mode q ζ' tx'),
         (λ vret, ∃ f t (LT : Time.lt f t) V' ζ'' ζn,
           let 𝓥' := TView.write_tview 𝓥 loc t ord in
@@ -167,7 +167,7 @@ Module SystemA. Section SystemA.
           own_writer γ mode q ζ'' (if mode is SingleWriter then t else tx') ∗
           @{TView.cur 𝓥'} loc sy⊒{γ} Cell.singleton (Message.message val V' false) LT ∗
           @{Vb ⊔ TView.cur 𝓥'} AtomicPtsToX loc γ (if mode is SingleWriter then t else tx') ζn mode ∗
-          tview_sys tid 𝓥')))%I.
+          tview_sys tid stid 𝓥')))%I.
 
   Definition write_spec : fspec := app_fspec [write_spec_0; write_spec_1].
 
@@ -183,28 +183,54 @@ Module SystemA. Section SystemA.
 
   (* Module definitions *)
   Definition scopes := ["System"].
-  Definition v_internal := "System" ↯ "internal".
+  Definition v_tid := "System" ↯ "tid".
+  Definition v_tids := "System" ↯ "tids".
 
-  (* Parameterized functions *)
-  Definition check_internal : itree crisE unit :=
-    _internal <- cgetU v_internal;;
-    assume (_internal = true);;;
-    cput v_internal false.
+  Definition _spawn : Ident.t * string * SAny.t → itree crisE unit :=
+    λ '(my_tid, fn, arg),
+      trigger (Call fn arg↑);;;
+      System.terminate.
 
-  Definition trigger_Yield (nxt_tid : Ident.t) : itree crisE unit :=
-    cput v_internal true;;;
-    SystemI.trigger_Yield nxt_tid;;;
-    check_internal.
+  Definition spawn : string * SAny.t → itree crisE unit :=
+    λ '(fn, arg),
+      'my_tid : Ident.t <- cgetN v_tid;;
+      'tids : tidmap <- cgetN v_tids;;
+      '(exist _ tid_new _) : _ <- trigger (Choose ({tid_new : Ident.t | tids !! tid_new = None}));;
+      (* 'new_mtid : Ident.t <- ccallN PFMemHdr.spawn my_tid;; *)
+      stid <- trigger (Spawn SystemHdr._spawn (tid_new, fn, arg)↑);;
+      let newtids : tidmap := <[tid_new := stid]> tids in
+      cput v_tids newtids.
 
-  Definition new_tid (tids : tidmap) (tid : Ident.t) : itree crisE Ident.t :=
-    '(exist _ tid_new _) : _ <- trigger (Choose ({tid_new : Ident.t | tids !! tid_new = None}));;
-    Ret tid_new.
+  Definition yield : unit → itree crisE unit :=
+    λ _,
+      'tids : tidmap <- cgetN v_tids;;
+      '(exist _ (mtid, stid) _) : _ <- trigger (Choose {p : Ident.t * nat | tids !! p.1 = Some p.2});;
+      cput v_tid mtid;;;
+      trigger (Yield stid).
+
+  Definition get_tid : () → itree crisE Ident.t :=
+    λ _, cgetN v_tid.
+
+  Definition alloc : nat → itree crisE Val.t :=
+    λ sz,
+      'tid : Ident.t <- get_tid ();;
+      ccallN PFMemHdr.alloc (tid, Z.of_nat sz).
+
+  Definition write : Loc.t * Val.t * Ordering.t → itree crisE Val.t :=
+    λ '(loc, val, ord),
+      'tid : Ident.t <- get_tid ();;
+      ccallN PFMemHdr.write (tid, loc, val, ord).
+
+  Definition read : Loc.t * Ordering.t → itree crisE Val.t :=
+    λ '(loc, ord),
+      'tid : Ident.t <- get_tid ();;
+      ccallN PFMemHdr.read (tid, loc, ord).
 
   Definition fnsems : alist (option string) (fnsem_type (option fspec * fbody)) :=
-    [(Some SystemHdr._spawn,  (true, wmask_all, scopes, (Some _spawn_spec,    (cfunN (SystemI._spawn check_internal)))));
-     (Some SystemHdr.spawn,   (true, wmask_all, scopes, (Some (spawn_spec ⊤), (cfunN (SystemI.spawn new_tid)))));
-     (Some SystemHdr.yield,   (true, wmask_all, scopes, (Some (yield_spec ⊤), (cfunN (SystemI.yield trigger_Yield)))));
-     (Some SystemHdr.get_tid, (true, wmask_all, scopes, (Some get_tid_spec,   (cfunN SystemI.get_tid))));
+    [(Some SystemHdr._spawn,  (true, wmask_all, scopes, (Some _spawn_spec,    (cfunN _spawn))));
+     (Some SystemHdr.spawn,   (true, wmask_all, scopes, (Some (spawn_spec ⊤), (cfunN spawn))));
+     (Some SystemHdr.yield,   (true, wmask_all, scopes, (Some (yield_spec ⊤), (cfunN yield))));
+     (Some SystemHdr.get_tid, (true, wmask_all, scopes, (Some get_tid_spec,   (cfunN get_tid))));
      (Some SystemHdr.alloc,   (true, wmask_all, scopes, (Some alloc_spec,     fbody_trivial)));
      (Some SystemHdr.write,   (true, wmask_all, scopes, (Some write_spec,     fbody_trivial)));
      (Some SystemHdr.read,    (true, wmask_all, scopes, (Some read_spec,      fbody_trivial)))].
@@ -212,13 +238,14 @@ Module SystemA. Section SystemA.
   Program Definition Mod : SMod.t := {|
     SMod.scopes := scopes;
     SMod.fnsems := fnsems;
-    SMod.initial_st := (v_internal, false↑) :: SystemI.Mod.(SMod.initial_st);
+    SMod.initial_st := 
+      [(v_tid, 1%positive↑); (v_tids, ({[1%positive := 0]} : tidmap)↑)];
   |}.
   Solve All Obligations with prove_scope.
   Next Obligation. prove_nodup. Qed.
 
   Definition init_cond size : iProp Σ :=
-    tview_sys_auth {[1%positive := TView.init size]}.
+    tview_sys_auth {[1%positive := (TView.init size, 0)]}.
 
   Definition t sp : Mod.t := Seal.sealing CRIS (SMod.to_mod sp Mod).
 End SystemA. End SystemA.
