promise_free/system/SystemI.v
@@ -4,37 +4,32 @@ Require Import SystemHeader PFMemHeader.
 Definition tidmap : Type := gmap Ident.t nat.
 
 Module SystemI. Section SystemI.
-  Context `{!crisG Γ Σ α β τ _S _I}.
+  Context `{!crisG Γ Σ α β τ _S _I, !concG}.
 
   Definition scopes := ["System"].
   Definition v_tid := "System" ↯ "tid".
   Definition v_tids := "System" ↯ "tids".
 
-  Definition _spawn
-      (check_internal : itree crisE unit)
-      : Ident.t * string * SAny.t → itree crisE unit :=
+  Definition _spawn : Ident.t * string * SAny.t → itree crisE unit :=
     λ '(my_tid, fn, arg),
-      check_internal;;;
-      cput v_tid my_tid;;;
       trigger (Call fn arg↑);;;
       System.terminate.
 
-  Definition spawn
-      (new_tid : tidmap → Ident.t → itree crisE Ident.t)
-      : string * SAny.t → itree crisE unit :=
+  Definition spawn : string * SAny.t → itree crisE unit :=
     λ '(fn, arg),
       'my_tid : Ident.t <- cgetU v_tid;;
       'tids : tidmap <- cgetU v_tids;;
-      'new_mtid : Ident.t <- new_tid tids my_tid;;
+      'new_mtid : Ident.t <- ccallU PFMemHdr.spawn my_tid;;
       new_stid <- trigger (Spawn SystemHdr._spawn (new_mtid, fn, arg)↑);;
       let newtids : tidmap := <[new_mtid := new_stid]> tids in
       cput v_tids newtids.
 
-  Definition yield (trigger_yield : Ident.t → itree crisE unit) : unit → itree crisE unit :=
+  Definition yield : unit → itree crisE unit :=
     λ _,
       'tids : tidmap <- cgetU v_tids;;
-      '(exist _ tid _) : _ <- trigger (Choose {tid : Ident.t | tid ∈ dom tids});;
-      trigger_yield tid.
+      '(exist _ (mtid, stid) _) : _ <- trigger (Choose {p : Ident.t * nat | tids !! p.1 = Some p.2});;
+      cput v_tid mtid;;;
+      trigger (Yield stid).
 
   Definition get_tid : () → itree crisE Ident.t :=
     λ _, cgetU v_tid.
@@ -54,27 +49,10 @@ Module SystemI. Section SystemI.
       'tid : Ident.t <- get_tid ();;
       ccallU PFMemHdr.read (tid, loc, ord).
 
-  (* Parameterized functions *)
-  Definition check_internal : itree crisE unit := Ret tt. (* skip *)
-
-  (* provide conversion between module-tid and system-tid *)
-  Definition trigger_Yield (nxt_mtid : Ident.t) : itree crisE unit :=
-    'my_tid : Ident.t <- cgetU v_tid;;
-    'tids : tidmap <- cgetU v_tids;;
-    match tids !! nxt_mtid with
-    | Some nxt_stid => 
-       trigger (Yield nxt_stid);;;
-       cput v_tid my_tid
-    | None => triggerUB
-    end.
-
-  Definition new_tid (_ : tidmap) (tid : Ident.t) : itree crisE Ident.t :=
-    ccallU PFMemHdr.spawn tid.
-
   Definition fnsems : alist (option string) (fnsem_type (option fspec * fbody)) :=
-    [(Some SystemHdr._spawn,  (false, wmask_all, scopes, (None, cfunU (_spawn check_internal))));
-     (Some SystemHdr.spawn,   (false, wmask_all, scopes, (None, cfunU (spawn new_tid))));
-     (Some SystemHdr.yield,   (false, wmask_all, scopes, (None, cfunU (yield trigger_Yield))));
+    [(Some SystemHdr._spawn,  (false, wmask_all, scopes, (None, cfunU _spawn)));
+     (Some SystemHdr.spawn,   (false, wmask_all, scopes, (None, cfunU spawn)));
+     (Some SystemHdr.yield,   (false, wmask_all, scopes, (None, cfunU yield)));
      (Some SystemHdr.get_tid, (false, wmask_all, scopes, (None, cfunU get_tid)));
      (Some SystemHdr.alloc,   (false, wmask_all, scopes, (None, cfunU alloc)));
      (Some SystemHdr.write,   (false, wmask_all, scopes, (None, cfunU write)));
