promise_free/system/SystemIAAlloc.v
@@ -4,7 +4,7 @@ Require Import PFMemHeader PFMemA HistoryRA AtomicRA.
 
 Section SystemIA.
   Import SystemA.
-  Context `{!crisG Γ Σ α β τ _S _I, !histG, !atomicG, !sysG}.
+  Context `{!crisG Γ Σ α β τ _S _I, !concG, !histG, !atomicG, !sysG}.
   Context (sp_user : spl_type).
   Context (sp : sp_type).
   Context (size : list Z).
@@ -17,14 +17,13 @@ Section SystemIA.
 
   Definition Ist : alist key Any.t → alist key Any.t → iProp Σ :=
     λ st_src st_tgt,
-      (∃ (tid : Ident.t) (tids : gmap Ident.t (TView.t * nat)) (flag : bool),
+      (∃ (tid : Ident.t) (tids : gmap Ident.t (TView.t * nat)),
         let tids' : gmap Ident.t nat := snd <$> tids in
         ⌜st_tgt = [(SystemI.v_tid, tid↑); (SystemI.v_tids, tids'↑)] ∧
-         st_src = [(v_internal, flag↑); (SystemI.v_tid, tid↑); (SystemI.v_tids, tids'↑)]⌝ ∗
-        (if flag then winv (⊤, ⊤) else True) ∗
-        tview_sys_auth (fst <$> tids) ∗
-        [∗ map] tid ↦ 𝓥 ∈ fst <$> (if flag then tids else delete tid tids),
-          tview_sys_gen (1/2) tid 𝓥)%I.
+         st_src = [(SystemA.v_tid, tid↑); (SystemA.v_tids, tids'↑)]⌝ ∗
+        tview_sys_auth tids ∗
+        ([∗ map] i ↦ stid ∈ (snd <$> delete tid tids),
+          (YIELD stid)))%I.
 
   Local Definition IstFull := (IstProd (IstSB (Mod.scopes (SystemA.t sp_user sp)) Ist) IstEq).
 
@@ -33,45 +32,41 @@ Section SystemIA.
     init_simF.
     steps_l. iDestruct "ASM" as "[[-> TVS] ->]".
     iDestruct "IST" as (????) "[[-> ->] [[% IST] ->]]".
-    iDestruct "IST" as "[%tid_cur [%tids [%flag [[-> ->] [W [[TA TVM] TVSM]]]]]]".
-    iPoseProof (tview_sys_lookup with "[TA TVM] TVS") as "%Hlookup"; first iFrame.
-    rename _q2 into V, _q3 into tid, _q4 into sz.
-    destruct (decide (tid = tid_cur)); cycle 1.
-    { iPoseProof (big_sepM_lookup_acc with "TVSM") as "[TV2 TVSM]".
-      { destruct flag; eauto. by rewrite fmap_delete lookup_delete_ne. }
-      iCombine "TVS TV2" gives %[WF _]%gmap_view.gmap_view_frag_op_valid.
-      by apply dfrac_valid_own in WF.
+    iDestruct "IST" as "[%tid_cur [%tids [[-> ->] [TA YS]]]]".
+    iDestruct "TVS" as "[Tid STV]".
+
+    (* Current tid is my tid *)
+    iPoseProof (tview_sys_lookup with "TA Tid") as "%Hlookup"; first iFrame.
+    destruct (decide (_q5 = tid_cur)); cycle 1.
+    { iPoseProof (big_sepM_lookup_acc with "YS") as "[TV2 YS]".
+      { instantiate (2:=_q5). rewrite lookup_fmap lookup_delete_ne // Hlookup; ss. }
+      iDestruct "STV" as "[_ Y2]"; iPoseProof (YieldToken_both with "Y2 TV2") as "%"; done.
     }
     subst.
-    destruct flag.
-    { iPoseProof (big_sepM_lookup_acc with "TVSM") as "[TVS2 TVSM]"; eauto.
-      iCombine "TVS TVS2" gives %[WF _]%gmap_view.gmap_view_frag_op_valid.
-      by apply dfrac_valid_own in WF.
-    }
+
     steps_r. hss_r. steps_r. rewrite /SystemI.get_tid. steps_r. hss_r. steps_r.
-    inline_r. force_r (tid_cur, sz, V). forces_r.
-    rewrite big_sepM_delete //. iDestruct "TVM" as "[$ TVM]"; eauto.
+    inline_r. force_r (_, _, _). forces_r.
+    iDestruct "TA" as "[TA TVS]".
+    rewrite big_sepM_delete //. iDestruct "TVS" as "[$ TVS]"; eauto.
     iSplit; eauto.
     steps_r. iDestruct "GRT" as "[[%loc [%V' [[-> %] [TV [FA MT]]]]] ->]".
-    iCombine "TA" "TVS" as "TA".
+    iCombine "TA" "Tid" as "TA".
     iMod (own_update with "TA") as "TA".
-    { rewrite (gmap_view_replace _ tid_cur _ (to_agree V')) //. }
-    iDestruct "TA" as "[TA TVS]". 
+    { rewrite (gmap_view_replace _ tid_cur _ (to_agree _)) //. }
+    iDestruct "TA" as "[TA Tid]". 
     hss_r. steps_r.
     forces_l. iFrame. iSplit; eauto.
     step.
+
+    (* IST *)
     iSplit; eauto.
-    iExists [_; _; _], [_; _], _, _; iSplit; eauto.
+    iExists [_; _], [_; _], _, _; iSplit; eauto.
     iSplit; eauto.
     iSplit; eauto.
-    rewrite lookup_fmap_Some in Hlookup; destruct Hlookup as [[? tid_s] [? Hlookup]]; ss; subst.
-    iExists tid_cur, (<[tid_cur := (V', tid_s)]> tids), _; iSplit.
+    iExists tid_cur, (<[tid_cur := (V', _)]> tids); iSplit.
     { iPureIntro; rewrite ?fmap_insert /= ?insert_id // lookup_fmap Hlookup //. }
-    rewrite fmap_insert /=; iFrame. iSplit; eauto.
-    iSplitL "TA TVM TV".
-    { rewrite /tview_sys_auth fmap_insert; iFrame.
-      rewrite big_sepM_insert_delete; iFrame.
-    }
-    { rewrite delete_insert_delete //=. }
+    rewrite -fmap_insert /=; iFrame. rewrite delete_insert_delete.
+    iSplitL "TVS TV"; eauto.
+    rewrite big_sepM_insert_delete; iFrame.
   Qed.
 End SystemIA.
