promise_free/system/SystemIARead.v
@@ -4,7 +4,7 @@ Require Import PFMemHeader PFMemA HistoryRA AtomicRA.
 
 Section SystemIA.
   Import SystemA.
-  Context `{!crisG Γ Σ α β τ _S _I, !histG, !atomicG, !sysG}.
+  Context `{!crisG Γ Σ α β τ _S _I, !concG, !histG, !atomicG, !sysG}.
   Context (sp_user : spl_type).
   Context (sp : sp_type).
   Context (size : list Z).
@@ -17,6 +17,16 @@ Section SystemIA.
 
   Definition Ist : alist key Any.t → alist key Any.t → iProp Σ :=
     λ st_src st_tgt,
+      (∃ (tid : Ident.t) (tids : gmap Ident.t (TView.t * nat)),
+        let tids' : gmap Ident.t nat := snd <$> tids in
+        ⌜st_tgt = [(SystemI.v_tid, tid↑); (SystemI.v_tids, tids'↑)] ∧
+         st_src = [(SystemA.v_tid, tid↑); (SystemA.v_tids, tids'↑)]⌝ ∗
+        tview_sys_auth tids ∗
+        ([∗ map] i ↦ stid ∈ (snd <$> delete tid tids),
+          (YIELD stid)))%I.
+
+  (* Definition Ist : alist key Any.t → alist key Any.t → iProp Σ :=
+    λ st_src st_tgt,
       (∃ (tid : Ident.t) (tids : gmap Ident.t (TView.t * nat)) (flag : bool),
         let tids' : gmap Ident.t nat := snd <$> tids in
         ⌜st_tgt = [(SystemI.v_tid, tid↑); (SystemI.v_tids, tids'↑)] ∧
@@ -24,7 +34,7 @@ Section SystemIA.
         (if flag then winv (⊤, ⊤) else True) ∗
         tview_sys_auth (fst <$> tids) ∗
         [∗ map] tid ↦ 𝓥 ∈ fst <$> (if flag then tids else delete tid tids),
-          tview_sys_gen (1/2) tid 𝓥)%I.
+          tview_sys_gen (1/2) tid 𝓥)%I. *)
 
   Local Definition IstFull := (IstProd (IstSB (Mod.scopes (SystemA.t sp_user sp)) Ist) IstEq).
 
@@ -32,55 +42,62 @@ Section SystemIA.
   Proof.
     init_simF.
     steps_l. destruct _q as [[|[|i]] X]; steps_l; rename _q0 into arg'.
-    { ss; destruct X as [[[[[tid loc] ord] val] q] V]; ss.
-      iDestruct "ASM" as "[[-> [PT TVS]] ->]".
+    { ss; destruct X as [[[[[[tid stid] loc] ord] val] q] V]; ss.
+      iDestruct "ASM" as "[[-> [PT TV]] ->]".
+      iDestruct "TV" as "[TV STV]".
       iDestruct "IST" as (????) "[[-> ->] [[% IST] ->]]".
-      iDestruct "IST" as "[%tid_cur [%tids [%flag [[-> ->] [W [[TA TVM] TVSM]]]]]]".
-      iPoseProof (tview_sys_lookup with "[TA TVM] TVS") as "%Hlookup"; first iFrame.
+      iDestruct "IST" as "[%tid_cur [%tids [[-> ->] [TA YS]]]]".
+      iPoseProof (tview_sys_lookup with "TA TV") as "%Hlookup"; first iFrame.
       destruct (decide (tid = tid_cur)); cycle 1.
-      { iPoseProof (big_sepM_lookup_acc with "TVSM") as "[TV2 TVSM]".
-        { destruct flag; eauto. by rewrite fmap_delete lookup_delete_ne. }
-        iCombine "TVS TV2" gives %[WF _]%gmap_view.gmap_view_frag_op_valid.
-        by apply dfrac_valid_own in WF.
+      { iPoseProof (big_sepM_lookup_acc with "YS") as "[TV2 YS]".
+        { instantiate (2:=tid). rewrite lookup_fmap lookup_delete_ne // Hlookup; ss. }
+        iDestruct "STV" as "[_ Y2]"; iPoseProof (YieldToken_both with "Y2 TV2") as "%"; done.
       }
       subst.
-      destruct flag.
+      (* destruct flag.
       { iPoseProof (big_sepM_lookup_acc with "TVSM") as "[TVS2 TVSM]"; eauto.
         iCombine "TVS TVS2" gives %[WF _]%gmap_view.gmap_view_frag_op_valid.
         by apply dfrac_valid_own in WF.
-      }
+      } *)
       steps_r. hss_r. steps_r. rewrite /SystemI.get_tid. steps_r. hss_r. steps_r.
       inline_r. force_r (existT 0 _). forces_r.
       instantiate (1 := (tid_cur, loc, ord, val, q, V)); ss; iFrame.
-      rewrite big_sepM_delete //. iDestruct "TVM" as "[$ TVM]"; eauto.
+      iDestruct "TA" as "[TA TVS]".
+      rewrite big_sepM_delete //=. iDestruct "TVS" as "[$ TVS]"; eauto.
       iSplit; eauto.
-      steps_r. iDestruct "GRT" as "[[%v [%V' [[-> %] [↦ TV]]]] ->]".
-      iCombine "TA" "TVS" as "TA".
+      steps_r. iDestruct "GRT" as "[[%v [%V' [[-> %] [↦ tv]]]] ->]".
+      iCombine "TA" "TV" as "TA".
       iMod (own_update with "TA") as "TA".
       { rewrite (gmap_view_replace _ tid_cur _ (to_agree _)) //. }
-      iDestruct "TA" as "[TA TVS]". 
+      iDestruct "TA" as "[TA TidS]". 
       hss_r. steps_r.
       forces_l. iFrame. iSplit; eauto.
       step.
       iSplit; eauto.
-      iExists [_; _; _], [_; _], _, _; iSplit; eauto.
+      iExists [_; _], [_; _], _, _; iSplit; eauto.
       iSplit; eauto.
       iSplit; eauto.
-      rewrite lookup_fmap_Some in Hlookup; destruct Hlookup as [[? tid_s] [? Hlookup]]; ss; subst.
-      iExists tid_cur, (<[tid_cur := (V', tid_s)]> tids), _; iSplit.
+      (* rewrite lookup_fmap_Some in Hlookup; destruct Hlookup as [[? tid_s] [? Hlookup]]; ss; subst. *)
+      iExists tid_cur, (<[tid_cur := (V', stid)]> tids); iSplit.
       { iPureIntro; rewrite ?fmap_insert /= ?insert_id // lookup_fmap Hlookup //. }
-      rewrite fmap_insert /=; iFrame. iSplit; eauto.
-      iSplitL "TA TVM TV".
-      { rewrite /tview_sys_auth fmap_insert; iFrame.
-        rewrite big_sepM_insert_delete; iFrame.
-      }
-      { rewrite delete_insert_delete //=. }
+      rewrite -fmap_insert /=; iFrame. rewrite delete_insert_delete.
+      iSplitL "TVS tv"; eauto.
+      rewrite big_sepM_insert_delete; iFrame.
     }
     { ss.
-      destruct X as [[[[[[[[[[tid loc] ord] ζ] ζ'] t0] γ] tx] mode] 𝓥] Vb]; ss.
-      iDestruct "ASM" as "[[[-> %] [PT [PTS TVS]]] ->]".
+      destruct X as [[[[[[[[[[[tid stid] loc] ord] ζ] ζ'] t0] γ] tx] mode] V] Vb].
+      ss; unfold_pre_post.
+      iDestruct "ASM" as "[[[-> %] [SN [PTS [Tid STid]]]] ->]".
       iDestruct "IST" as (????) "[[-> ->] [[% IST] ->]]".
-      iDestruct "IST" as "[%tid_cur [%tids [%flag [[-> ->] [W [[TA TVM] TVSM]]]]]]".
+      iDestruct "IST" as "[%tid_cur [%tids [[-> ->] [TA YS]]]]". hss_r. steps_r.
+      iPoseProof (tview_sys_lookup with "TA Tid") as "%Hlookup"; first iFrame.
+      destruct (decide (tid = tid_cur)); cycle 1.
+      { iPoseProof (big_sepM_lookup_acc with "YS") as "[TV2 YS]".
+        { instantiate (2:=tid). rewrite lookup_fmap lookup_delete_ne // Hlookup; ss. }
+        iDestruct "STid" as "[_ Y2]"; iPoseProof (YieldToken_both with "Y2 TV2") as "%"; done.
+      }
+      subst.
+      (* iDestruct "IST" as "[%tid_cur [%tids [%flag [[-> ->] [W [[TA TVM] TVSM]]]]]]".
       iPoseProof (tview_sys_lookup with "[TA TVM] TVS") as "%Hlookup"; first iFrame.
       destruct (decide (tid = tid_cur)); cycle 1.
       { iPoseProof (big_sepM_lookup_acc with "TVSM") as "[TV2 TVSM]".
@@ -88,39 +105,38 @@ Section SystemIA.
         iCombine "TVS TV2" gives %[WF _]%gmap_view.gmap_view_frag_op_valid.
         by apply dfrac_valid_own in WF.
       }
-      subst.
-      destruct flag.
+      subst. *)
+      (* destruct flag.
       { iPoseProof (big_sepM_lookup_acc with "TVSM") as "[TVS2 TVSM]"; eauto.
         iCombine "TVS TVS2" gives %[WF _]%gmap_view.gmap_view_frag_op_valid.
         by apply dfrac_valid_own in WF.
-      }
-      steps_r. hss_r. steps_r. rewrite /SystemI.get_tid. steps_r. hss_r. steps_r.
+      } *)
+      (* steps_r. hss_r. steps_r. *)
+      rewrite /SystemI.get_tid. steps_r. hss_r. steps_r.
       inline_r. force_r (existT 1 (tid_cur, loc, ord, _, _, _, _, _, _, _, _)).
       forces_r. iFrame.
-      rewrite big_sepM_delete //. iDestruct "TVM" as "[$ TVM]"; eauto.
+      iDestruct "TA" as "[TA TVS]".
+      rewrite big_sepM_delete //. iDestruct "TVS" as "[$ TVS]"; eauto.
       iSplit; eauto.
       steps_r. iDestruct "GRT" as "[[% [% [% [% [% [% [% [[-> %] [SN [PTS TV]]]]]]]]]] ->]".
-      iCombine "TA" "TVS" as "TA".
+      iCombine "TA" "Tid" as "TA".
       iMod (own_update with "TA") as "TA".
       { rewrite (gmap_view_replace _ tid_cur _ (to_agree _)) //. }
-      iDestruct "TA" as "[TA TVS]". 
+      iDestruct "TA" as "[TA Tid]". 
       hss_r. steps_r.
       forces_l. iFrame. iSplit; eauto. iSplit; eauto.
       iPureIntro; des; esplits; eauto.
       step.
       iSplit; eauto.
-      iExists [_; _; _], [_; _], _, _; iSplit; eauto.
+      iExists [_; _], [_; _], _, _; iSplit; eauto.
       iSplit; eauto.
       iSplit; eauto.
-      rewrite lookup_fmap_Some in Hlookup; destruct Hlookup as [[? tid_s] [? Hlookup]]; ss; subst.
-      iExists tid_cur, (<[tid_cur := (_, tid_s)]> tids), _; iSplit.
+      (* rewrite lookup_fmap_Some in Hlookup; destruct Hlookup as [[? tid_s] [? Hlookup]]; ss; subst. *)
+      iExists tid_cur, (<[tid_cur := (_, stid)]> tids); iSplit.
       { iPureIntro; rewrite ?fmap_insert /= ?insert_id // lookup_fmap Hlookup //. }
-      rewrite fmap_insert /=; iFrame. iSplit; eauto.
-      iSplitL "TA TVM TV".
-      { rewrite /tview_sys_auth fmap_insert; iFrame.
-        rewrite big_sepM_insert_delete; iFrame.
-      }
-      { rewrite delete_insert_delete //=. }
+      rewrite -fmap_insert /=; iFrame. rewrite delete_insert_delete.
+      iSplitL "TVS TV"; eauto.
+      rewrite big_sepM_insert_delete; iFrame.
     }
     { destruct i; ss. }
   Unshelve. exact 1%Qp.
